test_subst_eqn.lean
@@ -1,5 +1,0 @@
-import Metamath.Verify
-
-#check Verify.Formula.subst.eq_1
-#check Verify.Formula.subst_def  
-#print Verify.Formula.subst
