test_duplicate_float.mm
@@ -1,5 +1,0 @@
-$c wff $.
-$v x $.
-
-wff-x $f wff x $.
-bad-float $f wff x $.
