test_nested_scopes.mm
@@ -1,9 +1,0 @@
-$c wff $.
-$v x $.
-
-${
-  wff-x1 $f wff x $.
-  ${
-    wff-x2 $f wff x $.
-  $}
-$}
